relation proofs stuck on clocking mismatches

compiler/backend/languages/semantics/thunkLangRelScript.sml
@@ -1,613 +1,166 @@
 open HolKernel Parse BasicProvers boolLib bossLib listTheory;
-open thunkLangTheory thunkLang_primitivesTheory thunkLangRel_primitivesTheory;
+open thunkLangTheory thunkLang_primitivesTheory 
+     thunkLangRel_primitivesTheory thunkLangRel_semanticsTheory;
 
 val _ = new_theory "thunkLangRel";
 val _ = numLib.prefer_num ();
 
-Definition fix_state_def:
-  fix_state s1 (res, s2) =
-    if s1.c < s2.c then (res, s1) else (res, s2)
-End
-
-Theorem fix_state_non_incr_thm:
-  ∀s1 s2 x res.
-   fix_state s1 x = (res, s2) ⇒ s2.c ≤ s1.c
-Proof
-  Cases_on `x` >> rw [fix_state_def] >> rw []
-QED
-
-Definition check_state_def:
-  check_state s e f =
-    if (s.c < fuel e) ∨ (s.t < trace e) then
-      (OOT, s)
-    else
-      f $ s - (state (fuel e) (trace e))
-End
-
-Theorem check_state_CONG[defncong]:
-  ∀s1 e1 s2 e2 f1 f2.
-   s1 = s2 ∧ e1 = e2
-   ∧ (∀s'. s'.c < s1.c ⇒ f1 s' = f2 s')
-   ⇒ check_state s1 e1 f1 = check_state s2 e2 f2
-Proof
-  rw [check_state_def, fuel_def]
-QED
-
-Definition dest_Closure'_def[simp]:
-  (dest_Closure' (Closure s x) = SOME (s, x)) ∧
-  (dest_Closure' _ = NONE)
-End
-
-Definition dest_Recclosure'_def[simp]:
-  (dest_Recclosure' (Recclosure f n) = SOME (f, n)) ∧
-  (dest_Recclosure' _ = NONE)
-End
-
-Definition dest_anyClosure'_def:
-  dest_anyClosure' v =
-    case dest_Closure' v of
-    | SOME (s, x) => SOME (s, x, [])
-    | NONE =>
-        (case dest_Recclosure' v of
-         | SOME (f, n) =>
-            (case ALOOKUP (REVERSE f) n of
-             | SOME (Lam s x) => SOME (s, x, MAP (λ(g, x). (g, Recclosure f g)) f)
-             | _ => NONE)
-         | NONE => NONE)
-End
-
-Definition dest_Tick'_def[simp]:
-  (dest_Tick' (DoTick v) = SOME v) ∧
-  (dest_Tick' _ = NONE)
-End
-
-Definition dest_Thunk'_def[simp]:
-  (dest_Thunk' (Thunk x) = SOME x) ∧
-  (dest_Thunk' _ = NONE)
-End
-
-Definition dest_anyThunk'_def:
-  dest_anyThunk' v =
-    case dest_Thunk' v of
-    | SOME w => SOME (w, [])
-    | _ =>
-        (case dest_Recclosure' v of
-         | SOME (f, n) =>
-            (case ALOOKUP (REVERSE f) n of
-             | SOME (Delay x) => SOME (x, f)
-             | _ => NONE)
-         | NONE => NONE)
-End
-
-Definition dest_Constructor'_def[simp]:
-  (dest_Constructor' (Constructor s vs) = SOME (s, vs)) ∧
-  (dest_Constructor' _ = NONE)
-End
-
-Definition mapok_def:
-  mapok st rs =
-    case FIND (isfail ∘ FST) rs of
-    | SOME (Fail, st) => (Fail, st)
-    | NONE =>
-        (case FIND (isoot ∘ FST) rs of
-         | SOME (OOT, st) => (OOT, st)
-         | NONE => (Ok (MAP (outok ∘ FST) rs), st))
-End
-
-Theorem mapok_non_incr_lemma:
-  ∀st rs rs' st'.
-    mapok st rs = (rs', st')
-    ∧ (∀s. MEM s (MAP SND rs) ⇒ s.c ≤ st.c)
-    ⇒ st'.c ≤ st.c
-Proof
-  rw [mapok_def]
-  >> gvs [AllCaseEqs()]
-  >> imp_res_tac FIND_pred_thm >> gvs []
-  >> imp_res_tac FIND_MEM_thm >> gvs []
-  >> imp_res_tac MEM_MAP_SND_thm >> gvs []
-QED
-
-Theorem mapok_every_thm:
-  ∀s rs r s'.
-    mapok s rs = (Ok r, s') ⇒ EVERY (isok ∘ FST) rs
-Proof
-  rw [mapok_def]
-  >> gvs [AllCaseEqs(), EVERY_MEM] >> rpt strip_tac
-  >> Cases_on `FST e` >> gvs []
-  >> imp_res_tac FIND_pred_thm >> gvs []
-QED
-
-Theorem mapok_ok_thm:
-  ∀s rs r s'.
-    mapok s rs = (Ok r, s') ⇒ r = MAP (outok ∘ FST) rs
-Proof
-  rw [mapok_def]
-  >> gvs [AllCaseEqs()]
-  >> imp_res_tac FIND_pred_thm >> gvs []
-QED
-
-Theorem mapok_add_thm:
-  ∀(s : state) sp q r s'.
-    mapok s q = (Ok r, s')
-    ⇒ mapok (s + sp) (MAP (with_snd (λs. s + sp)) q)
-        = (Ok r, s' + sp)
-Proof
-  rw [mapok_def]
-  >> gvs [AllCaseEqs(), FIND_FST_WITH_SND_thm, MAP_FST_WITH_SND_thm]
-  >> imp_res_tac FIND_pred_thm >> gvs []
-QED
-
-Definition atom_lit_def:
-  atom_lit r =
-    case r of
-    | Ok (Atom l) => Ok l
-    | Ok _ => Fail
-    | Fail => Fail
-    | OOT => OOT
-End
-
-Theorem atom_lit_isok_thm:
-  ∀x. (isok ∘ atom_lit) x ⇒ isok x
-Proof
-  Cases_on `x` >> gvs [atom_lit_def]
-QED
-
-Theorem EVERY_atom_lit_thm:
-  ∀l.
-    EVERY (isok ∘ atom_lit ∘ FST) l
-    ⇒ EVERY (isok ∘ FST) l
-Proof
-  Induct_on `l` >> gvs []
-  >> rpt strip_tac
-  >> qspec_then `FST h` assume_tac atom_lit_isok_thm
-  >> gvs []
-QED
-
-Definition eval_to'_def:
-  (eval_to' st (Value v) =
-    check_state st (Value v) (λst.
-      (Ok v, st))) ∧
-  (eval_to' st (Var n) =
-    check_state st (Var n) (λst.
-      (Fail, st))) ∧
-  (eval_to' st (App f x) =
-    check_state st (App f x) (λst.
-      case fix_state st (eval_to' st x) of
-      | (Ok xv, st') =>
-          (case fix_state st' (eval_to' st' f) of
-           | (Ok fv, st'') =>
-               (case dest_anyClosure' fv of
-                | SOME (n, body, binds) =>
-                    let y = subst (binds ++ [(n, xv)]) body in
-                    eval_to' st'' y
-                | NONE => (Fail, st''))
-           | res => res)
-      | res => res)) ∧
-  (eval_to' st (Lam n x) =
-    check_state st (Lam n x) (λst.
-      (Ok (Closure n x), st))) ∧
-  (eval_to' st (Let NONE x y) =
-    check_state st (Let NONE x y) (λst.
-      case fix_state st (eval_to' st x) of
-      | (Ok xv, st') => eval_to' st' y
-      | res => res)) ∧
-  (eval_to' st (Let (SOME n) x y) =
-    check_state st (Let (SOME n) x y) (λst.
-      case fix_state st (eval_to' st x) of
-      | (Ok xv, st') => eval_to' st' (subst1 n xv y)
-      | res => res)) ∧
-  (eval_to' st (If x y z) =
-    check_state st (If x y z) (λst.
-      case fix_state st (eval_to' st x) of
-      | (Ok (Constructor "True" []), st') => eval_to' st' y
-      | (Ok (Constructor "False" []), st') => eval_to' st' z
-      | (Ok _, st') => (Fail, st')
-      | res => res)) ∧
-  (eval_to' st (Letrec funs x) =
-    check_state st (Letrec funs x) (λst.
-      eval_to' st (subst_funs funs x))) ∧
-  (eval_to' st (Delay x) =
-    check_state st (Delay x) (λst.
-      (Ok (Thunk x), st))) ∧
-  (eval_to' st (Force x) =
-    check_state st (Force x) (λst.
-      case fix_state st (eval_to' st x) of
-      | (Ok xv, st') =>
-          (case dest_anyThunk' xv of
-           | SOME (y, binds) =>
-               eval_to' st' (subst_funs binds y)
-           | NONE => (Fail, st'))
-      | res => res)) ∧
-  (eval_to' st (MkTick x) =
-    check_state st (MkTick x) (λst.
-      case fix_state st (eval_to' st x) of
-      | (Ok xv, st') => (Ok (DoTick xv), st')
-      | res => res)) ∧
-  (eval_to' st (Prim op xs) =
-    check_state st (Prim op xs) (λst.
-      (case op of
-       | If => (Fail, st)
-       | Seq => (Fail, st)
-       | Proj s i =>
-           if LENGTH xs ≠ 1 then
-             (Fail, st)
-           else
-             (case fix_state st (eval_to' st (HD xs)) of
-              | (Ok v, st') =>
-                  (case dest_Constructor' v of
-                   | SOME (t, ys) =>
-                       if (t ≠ s) ∨ (i ≥ LENGTH ys) then
-                         (Fail, st')
-                       else
-                         (Ok (EL i ys), st')
-                   | NONE => (Fail, st'))
-              | res => res)
-       | IsEq s i a =>
-           if LENGTH xs ≠ 1 then
-             (Fail, st)
-           else
-             (case fix_state st (eval_to' st (HD xs)) of
-              | (Ok v, st') =>
-                  (case dest_Constructor' v of
-                   | SOME (t, ys) =>
-                       if (¬(t = s ⇒ i = LENGTH ys)) ∨ (t ∈ monad_cns) then
-                         (Fail, st')
-                       else if t = s then
-                         (Ok (Constructor "True" []), st')
-                       else
-                         (Ok (Constructor "False" []), st')
-                   | NONE => (Fail, st'))
-              | res => res)
-       | AtomOp aop =>
-           let (rs, st') = result_map' st xs in
-           let rs = MAP (with_fst atom_lit) rs in
-           (case mapok st rs of
-            | (Fail, st') => (Fail, st')
-            | (OOT, st') => (OOT, st')
-            | (Ok vs, st') =>
-                (case eval_op aop vs of
-                 | SOME (INL v) =>
-                     (Ok (Atom v), st')
-                  | SOME (INR b) =>
-                      (Ok (Constructor (if b then "True" else "False") []), st')
-                  | NONE => (Fail, st')))
-       | Cons s =>
-           let (rs, st') = result_map' st xs in
-           (case mapok st rs of
-            | (Fail, st') => (Fail, st')
-            | (OOT, st') => (OOT, st')
-            | (Ok vs, st') => (Ok (Constructor s vs), st'))))) ∧
-  (eval_to' s (Monad mop xs) =
-    check_state s (Monad mop xs) (λs.
-      (Ok (Monadic mop xs), s))) ∧
-  (result_map' st [] = ([], st)) ∧
-  (result_map' st (x::xs) =
-    let (r, st') = fix_state st (eval_to' st x) in
-    let (rs, st'') = result_map' st' xs in
-    ((r, st') :: rs, st''))
-Termination
-  WF_REL_TAC `inv_image ($< LEX $<)
-                (λx. case x of
-                     | INL (s, e) => (s.c, exp_size e)
-                     | INR (s, es) => (s.c, list_size exp_size es))`
-  >> rw []
-  >> gvs []
-  >> imp_res_tac fix_state_non_incr_thm
-  >> imp_res_tac (GSYM fix_state_non_incr_thm)
-  >> gvs []
-End
-
-Theorem eval_to'_non_incr_thm:
-  (∀s e res s'.
-    eval_to' s e = (res, s') ⇒ s'.c ≤ s.c) ∧
-  (∀s xs rs s'.
-    result_map' s xs = (rs, s')
-    ⇒ (s'.c ≤ s.c
-       ∧ (∀st. MEM st (MAP SND rs) ⇒ st.c ≤ s.c)))
-Proof
-  ho_match_mp_tac eval_to'_ind
-  >> rw [eval_to'_def, check_state_def, fuel_def, trace_def]
-  >> gvs [AllCaseEqs()]
-  >> imp_res_tac fix_state_non_incr_thm >> gvs []
-  >>~- ([`mapok _ _`],
-        Cases_on `result_map' (state (s.c - 1) s.t) xs`
-        >> gvs [AllCaseEqs()]
-        >> imp_res_tac mapok_non_incr_lemma
-        >> gvs [MAP_SND_MAP_WITH_FST_thm])
-  >>~- ([`result_map' _ _`],
-        Cases_on `fix_state s (eval_to' s e)` >> gvs []
-        >> Cases_on `result_map' r xs` >> gvs []
-        >> imp_res_tac fix_state_non_incr_thm >> gvs []
-        >> res_tac >> simp [])
-  >> qmatch_asmsub_abbrev_tac `state a b`
-  >> rpt (last_x_assum $ qspec_then `state a b` assume_tac
-          >> gvs [])
-  >> unabbrev_all_tac >> gvs []
-QED
-
-Theorem fix_state_thm:
-  ∀s e. fix_state s (eval_to' s e) = eval_to' s e
-Proof
-  rpt strip_tac
-  >> Cases_on `eval_to' s e` >> rw [fix_state_def]
-  >> imp_res_tac eval_to'_non_incr_thm >> gvs []
-QED
-
-Theorem eval_to'_def[compute,allow_rebind] =
-  REWRITE_RULE [fix_state_thm] eval_to'_def;
-
-Theorem eval_to'_ind[allow_rebind] =
-  REWRITE_RULE [fix_state_thm] eval_to'_ind;
-
-Theorem eval_to'_add_lemma:
-  (∀s e res s' sp.
-    eval_to' s e = (Ok res, s')
-    ⇒ eval_to' (s + sp) e = (Ok res, s' + sp)) ∧
-  (∀s xs rs s' sp.
-    result_map' s xs = (rs, s')
-    ∧ EVERY (isok ∘ FST) rs
-    ⇒ result_map' (s + sp) xs = (MAP (with_snd (λs. s + sp)) rs, s' + sp))
-Proof
-  ho_match_mp_tac eval_to'_ind
-  >> rw [eval_to'_def, check_state_def, fuel_def, trace_def]
-  >> gvs [AllCaseEqs()]
-  >>~- ([`mapok _ _`],
-        Cases_on `result_map' (state (s.c - 1) s.t) xs`
-        >> first_x_assum $ qspec_then `state (s.c - 1) s.t` assume_tac
-        >> gvs [AllCaseEqs()]
-        >> imp_res_tac mapok_every_thm >> gvs []
-        >> imp_res_tac mapok_add_thm
-        >> gvs [EVERY_MAP_WITH_FST_thm, EVERY_atom_lit_thm,
-                MAP_WITH_FST_WITH_SND_thm])
-  >>~- ([`result_map' _ _`],
-        Cases_on `eval_to' s e` >> gvs []
-        >> Cases_on `result_map' r xs` >> gvs []
-        >> Cases_on `q` >> gvs [with_snd_def])
-  >> qmatch_asmsub_abbrev_tac `state a b`
-  >> rpt (first_x_assum $ qspec_then `state a b` assume_tac
-          >> gvs [])
-  >> unabbrev_all_tac >> gvs []
-QED
-
-Theorem eval_to'_add_thm:
-  (∀s sp e res s'.
-    eval_to' s e = (Ok res, s')
-    ⇒ eval_to' (s + sp) e = (Ok res, s' + sp)) ∧
-  (∀s sp xs rs s'.
-    result_map' s xs = (rs, s')
-    ∧ EVERY (isok ∘ FST) rs
-    ⇒ result_map' (s + sp) xs = (MAP (with_snd (λs. s + sp)) rs, s' + sp))
-Proof
-  rw [eval_to'_add_lemma]
-QED
-
-Theorem eval_to_add_thm:
-  ∀c c' e v.
-    eval_to c e = INR v
-    ⇒ eval_to (c + c') e = INR v
-Proof
-  rpt strip_tac
-  >> qspecl_then [`c`, `e`, `c + c'`] assume_tac eval_to_mono
-  >> rw []
-QED
-
-Theorem result_map_add_thm:
-  ∀c c' xs rs.
-    result_map (λx. eval_to c x) xs = INR rs
-    ⇒ result_map (λx. eval_to (c + c') x) xs = INR rs
-Proof
-  cheat
-QED
-
-Theorem eval_requiv_lemma:
-  (∀s e v s'.
-    eval_to' s e = (Ok v, s')
-    ⇒ ∃c. eval_to c e = INR v) ∧
-  (∀s xs rs s'.
-    result_map' s xs = (rs, s')
-    ∧ EVERY (isok ∘ FST) rs
-    ⇒ ∃c. result_map (λx. eval_to c x) xs = INR (MAP (outok ∘ FST) rs))
-Proof
-  ho_match_mp_tac eval_to'_ind
-  >> rw []
-  >> gvs [AllCaseEqs(), Once eval_to_def, eval_to'_def, check_state_def, fuel_def, trace_def]
-  >- (rpt (first_x_assum $ qspec_then `state (s.c - 1) (s.t + 1)` assume_tac
-           >> gvs [])
-      >> qexists `c + c' + c'' + 1`
-      >> qspecl_then [`c`, `c' + c'' + 1`] assume_tac eval_to_add_thm
-      >> pop_assum drule >> rw []
-      >> qspecl_then [`c'`, `c + c'' + 1`] assume_tac eval_to_add_thm
-      >> pop_assum drule >> rw []
-      >> Cases_on `fv` >> gvs [AllCaseEqs(), dest_anyClosure_def, dest_anyClosure'_def]
-      >> qspecl_then [`c''`, `c + c'`] assume_tac eval_to_add_thm
-      >> pop_assum drule >> rw [])
-  >- (rpt (first_x_assum $ qspec_then `state (s.c - 1) s.t` assume_tac
-           >> gvs [])
-      >> qexists `c + c' + 1`
-      >> qspecl_then [`c`, `c'`] assume_tac eval_to_add_thm
-      >> pop_assum drule >> rw []
-      >> qspecl_then [`c'`, `c`] assume_tac eval_to_add_thm
-      >> pop_assum drule >> rw [])
-  >- (rpt (first_x_assum $ qspec_then `state (s.c - 1) s.t` assume_tac
-           >> gvs [])
-      >> qexists `c + c' + 1`
-      >> qspecl_then [`c`, `c'`] assume_tac eval_to_add_thm
-      >> pop_assum drule >> rw []
-      >> qspecl_then [`c'`, `c`] assume_tac eval_to_add_thm
-      >> pop_assum drule >> rw [])
-  >- (gvs [Once eval_to_def]
-      >> rpt (first_x_assum $ qspec_then `state (s.c - 1) s.t` assume_tac
-              >> gvs [])
-      >> qexists `c + c' + 1`
-      >> qspecl_then [`c`, `c'`] assume_tac eval_to_add_thm
-      >> pop_assum drule >> rw []
-      >> qspecl_then [`c'`, `c`] assume_tac eval_to_add_thm
-      >> pop_assum drule >> rw [])
-  >- (gvs [Once eval_to_def]
-      >> rpt (first_x_assum $ qspec_then `state (s.c - 1) s.t` assume_tac
-              >> gvs [])
-      >> qexists `c + c' + 1`
-      >> qspecl_then [`c`, `c'`] assume_tac eval_to_add_thm
-      >> pop_assum drule >> rw []
-      >> qspecl_then [`c'`, `c`] assume_tac eval_to_add_thm
-      >> pop_assum drule >> rw [])
-  >- (rpt (first_x_assum $ qspec_then `state (s.c - 1) s.t` assume_tac
-           >> gvs [])
-      >> qexists `c + 1` >> gvs []) 
-  >- (rpt (first_x_assum $ qspec_then `state (s.c - 1) s.t` assume_tac
-           >> gvs [])
-      >> qexists `c + c' + 1` >> gvs []
-      >> qspecl_then [`c`, `c' + 1`] assume_tac eval_to_add_thm
-      >> pop_assum drule >> rw []
-      >> Cases_on `xv` >> gvs [AllCaseEqs(), dest_Tick_def, dest_anyThunk_def,
-                               dest_anyThunk'_def]
-      >> qspecl_then [`c'`, `c`] assume_tac eval_to_add_thm
-      >> pop_assum drule >> rw [])
-  >- (rpt (first_x_assum $ qspec_then `state (s.c - 1) s.t` assume_tac
-           >> gvs [])
-      >> qexists `c` >> gvs [])
-  >- (gvs [Once eval_to_def]
-      >> rpt (first_x_assum $ qspec_then `state (s.c - 1) s.t` assume_tac
-              >> gvs [])
-      >> Cases_on `result_map' (state (s.c - 1) s.t) xs` >> gvs []
-      >> ntac 2 (FULL_CASE_TAC >> gvs [])
-      >> imp_res_tac mapok_every_thm >> gvs []
-      >> qexists_tac `c` >> gvs []
-      >> imp_res_tac mapok_ok_thm >> gvs [])
-  >- (gvs [Once eval_to_def]
-      >> rpt (first_x_assum $ qspec_then `state (s.c - 1) s.t` assume_tac
-              >> gvs [])
-      >> qexists_tac `c + 1` >> gvs []
-      >> Cases_on `v'` >> gvs [AllCaseEqs(), dest_Constructor_def,
-                               dest_Constructor'_def])
-  >- (gvs [Once eval_to_def]
-      >> rpt (first_x_assum $ qspec_then `state (s.c - 1) s.t` assume_tac
-              >> gvs [])
-      >> qexists_tac `c + 1` >> gvs []
-      >> Cases_on `v'` >> gvs [AllCaseEqs(), dest_Constructor_def,
-                               dest_Constructor'_def])
-  >- (gvs [Once eval_to_def]
-      >> rpt (first_x_assum $ qspec_then `state (s.c - 1) s.t` assume_tac
-              >> gvs [])
-      >> qexists_tac `c + 1` >> gvs []
-      >> Cases_on `v'` >> gvs [AllCaseEqs(), dest_Constructor_def,
-                               dest_Constructor'_def])
-  >- cheat
-  >- gvs [result_map_def]
-  >- (Cases_on `eval_to' s e` >> gvs []
-      >> Cases_on `result_map' r xs` >> gvs []
-      >> Cases_on `q` >> gvs []
-      >> qexists_tac `c + c'`
-      >> qspecl_then [`c'`, `c`] assume_tac eval_to_add_thm
-      >> pop_assum drule >> rw []
-      >> imp_res_tac result_map_add_thm
-      >> first_x_assum $ qspec_then `c'` assume_tac
-      >> imp_res_tac result_map_INR
-      >> rw [result_map_INR, map_def])
-QED
-
-Theorem eval_lequiv_lemma:
-  ∀c e v.
-    eval_to c e = INR v
-    ⇒ ∃s s' . eval_to' s e = (Ok v, s')
-Proof
-  cheat
-QED
-
 Type inv = ``:state -> state -> bool``;
+Type sigma = ``:(string # v) list``;
 
 Definition rel_def:
-  (val_rel (s : state) (q : inv) (Constructor n vs) (Constructor n' vs') ⇔
-    n = n' ∧ LIST_REL (val_rel s q) vs vs') ∧
-  (val_rel s q (Monadic op es) (Monadic op' es') ⇔
-    op = op' ∧ LIST_REL (exp_rel s (q, q)) es es') ∧
-  (val_rel s q (Closure x e) (Closure x' e') ⇔
-    ∀s' v1 v2.
-      if s'.c < s.c then
-        val_rel s' q v1 v2
-        ⇒ exp_rel s' (q, q) (subst1 x v1 e) (subst1 x' v2 e')
-      else
-        T) ∧
-  (val_rel s q (Recclosure fs n) (Recclosure fs' n') ⇔
-    ∀s' e e'.
-      s'.c < s.c
+  (val_rel (k : fuel) (Q : inv) (Constructor n vs) (Constructor n' vs') ⇔
+    n = n'
+    ∧ LIST_REL (val_rel k Q) vs vs') ∧
+  (val_rel k Q (Monadic op es) (Monadic op' es') ⇔
+    op = op'
+    ∧ ∀i. i < k
+      ⇒ LIST_REL (exp_rel i (Q, Q)) es es') ∧
+  (val_rel k Q (Closure x e) (Closure x' e') ⇔
+    ∀i v1 v2.
+      i < k
+      ⇒ val_rel i Q v1 v2
+      ⇒ exp_rel i (Q, Q) (subst1 x v1 e) (subst1 x' v2 e')) ∧
+  (val_rel k Q (Recclosure fs n) (Recclosure fs' n') ⇔
+    ∀i e e'.
+      i < k
       ∧ ALOOKUP fs n = SOME e
       ∧ ALOOKUP fs' n' = SOME e'
-      ⇒
-      exp_rel s (q, q) (subst_funs fs e) (subst_funs fs' e')) ∧
-  (val_rel s q (Thunk e) (Thunk e') ⇔
-    exp_rel s (q, q) e e') ∧
-  (val_rel s q (Atom l) (Atom l') ⇔
-    l = l') ∧
-  (val_rel s q (DoTick v) (DoTick v') ⇔
-    val_rel s q v v') ∧
-  (val_rel s q v1 v2 ⇔ F) ∧
+      ⇒ exp_rel i (Q, Q) (subst_funs fs e) (subst_funs fs' e')) ∧
+  (val_rel k Q (Thunk e) (Thunk e') ⇔
+    ∀i. i < k ⇒ exp_rel i (Q, Q) e e') ∧
+  (val_rel k Q (Atom l) (Atom l') ⇔ l = l') ∧
+  (val_rel k Q (DoTick v) (DoTick v') ⇔ val_rel k Q v v') ∧
+  (val_rel k Q v1 v2 ⇔ F) ∧
 
-  (res_rel (s : state) (q : inv) OOT OOT ⇔ T) ∧
-  (res_rel s q Fail Fail ⇔ T) ∧
-  (res_rel s q (Ok v) (Ok v') ⇔
-    val_rel s q v v') ∧
-  (res_rel s q r1 r2 ⇔ F) ∧
+  (res_rel (k : fuel) (Q : inv) OOT OOT ⇔ T) ∧
+  (res_rel k Q Fail Fail ⇔ T) ∧
+  (res_rel k Q (Ok v) (Ok v') ⇔ val_rel k Q v v') ∧
+  (res_rel k Q r1 r2 ⇔ F) ∧
 
-  (exp_rel (s : state) ((ql, qg) : inv # inv) (e1 : exp) (e2 : exp) ⇔
-    ∀r1 s'.
-      s'.c ≤ s.c
-      ⇒ FST (eval_to' s' e1) = r1
-      ⇒ (∃r2 s''.
-          FST (eval_to' s'' e2) = r2 ∧
-          ql s' s'' ∧
-          res_rel <|c := s.c - s'.c; t := s.t|> qg r1 r2))
+  (exp_rel (k : fuel) ((QL, QG) : inv # inv) (e1 : exp) (e2 : exp) ⇔
+    ∀c1 t1 r1.
+      c1 ≤ k
+      ⇒ FST (eval_to' (state c1 t1) e1) = r1
+      ⇒ (∃c2 t2 r2.
+          FST (eval_to' (state c2 t2) e2) = r2
+          ∧ QL (state c1 t1) (state c2 t2)
+          ∧ res_rel (k - c1) QG r1 r2))
 Termination
-  cheat
-  (*WF_REL_TAC `inv_image ($< LEX ($< LEX $<))
-              (λx. case x of
-                   | INL (s, q, v1, v2) => (s.c, (v_size v1, 0))
-                   | INR (INL (s, q, r1, r2)) => (s.c, (res_size v_size r1, 1))
-                   | INR (INR (s, (ql,qg), e1, e2)) => (s.c, (exp_size e1, 2)))`*)
+  WF_REL_TAC `inv_image ($< LEX $< LEX $<) (λx.
+                case x of
+                | INL (k, q, v1, v2) => (k, 0, v_size v1)
+                | INR (INL (k, q, r1, r2)) => (k, 1, res_size v_size r1)
+                | INR (INR (k, (ql, qg), e1, e2)) => (k, 2, exp_size e1))`
+End
+
+Definition var_rel_def:
+  var_rel (k : fuel) (Q : inv) (sub1 : sigma) (sub2 : sigma)
+          (x : string) (y : string) ⇔
+    ∀v1. ALOOKUP sub1 x = SOME v1
+         ⇒ ∃v2. ALOOKUP sub2 y = SOME v2
+                ∧ val_rel k Q v1 v2
 End
 
 Definition subst_rel_def:
-  (subst_rel (s : state) (q : inv) (S : string set) (sub1 : (string # v) list) (sub2 : (string # v) list) ⇔  
-    ∀x v1.
-      if x ∈ S then
-        ALOOKUP sub1 x = SOME v1
-        ⇒ (∃v2. 
-            ALOOKUP sub2 x = SOME v2
-            ∧ val_rel s q v1 v2)
-      else
-        T)
+  subst_rel (k : fuel) (Q : inv) (S : string set)
+            (sub1 : sigma) (sub2 : sigma) ⇔
+    ∀x. x ∈ S ⇒ var_rel k Q sub1 sub2 x x
 End
 
 Definition top_rel_def:
-  top_rel ((ql, qg) : inv # inv) (e1 : exp) (e2 : exp) ⇔
-    ∀(s : state) (sub1 : (string # v) list) (sub2 : (string # v) list).
-      subst_rel s qg (freevars e1) sub1 sub2
+  top_rel ((QL, QG) : inv # inv) (e1 : exp) (e2 : exp) ⇔
+    ∀k sub1 sub2.
+      subst_rel k QG (freevars e1) sub1 sub2
       ⇒ (freevars e1) ⊆ (set (MAP FST sub1))
-      ⇒ exp_rel s (ql, qg) e1 e2
+      ⇒ exp_rel k (QL, QG) (subst sub1 e1) (subst sub2 e2)
 End
 
-Definition constr_compat_thm:
-    ∀st ql qg x1 x2 n1 n2 es1 es2.
-      ql (state 0 0) (state 0 0)
-      ∧ (∀s1 s2. ql s1 s2 ⇒ ql (s1 + (state 1 0)) (s2 + (state 1 0)))
-      ∧ ((∀vs1 vs2. LIST_REL (val_rel st qg) vs1 vs2
-          ⇒ exp_rel st (ql, qg) (subst1 x1 (Constructor n1 vs1) e1)
-                                (subst1 x2 (Constructor n2 vs2) e2)))
-      ⇒ exp_rel st (ql, qg) (Let (SOME x1) (Value $ Constructor n1 es1) e1)
-                            (Let (SOME x2) (Value $ Constructor n2 es2) e2)
+Theorem eval_to'_oot_thm:
+  ∀t e. eval_to' (state 0 t) e = (OOT, (state 0 t))
 Proof
-  gvs [rel_def]
-  >> gvs [AllCaseEqs(), eval_to'_def, check_state_def, fuel_def, trace_def]
-  >> rpt strip_tac
-  >> qexists `s'`
+  rw []
+  >> Cases_on `e`
+  >~ [`Let x _ _`]
+  >- (Cases_on `x`
+      >> gvs [eval_to'_def, check_state_def, fuel_def, trace_def])
+  >> gvs [eval_to'_def, check_state_def, fuel_def, trace_def]
+QED
+
+Theorem eval_to'_zero_thm:
+  ∀t e r s'.
+    eval_to' (state 0 t) e = (r, s')
+    ⇒ r = OOT
+Proof
+  cheat
+QED
+
+Theorem rel_add_thm:
+  (∀k c Q x x'.
+    val_rel (k + c) Q x x'
+    ⇒ val_rel k Q x x') ∧
+  (∀k c Q r r'.
+    res_rel (k + c) Q r r'
+    ⇒ res_rel k Q r r') ∧
+  (∀k c Qs e1 e2.
+    exp_rel (k + c) Qs e1 e2
+    ⇒ exp_rel k Qs e1 e2)
+Proof
+  cheat
+QED
+
+Theorem constr_compat_thm:
+  ∀(k : fuel) (QL : inv) (QG : inv)
+   (ys1 : string list) (ys2 : string list)
+   (x1 : string) (x2 : string) (sub1 : sigma)
+   (sub2 : sigma) (C : string)
+   (e1 : exp) (e2 : exp).
+    QL (state 0 0) (state 0 0)
+    ∧ (∀c1 t1 c2 t2.
+        QL (state c1 t1) (state c2 t2) 
+        ⇒ QL (state (c1 + 1) t1) (state (c2 + 1) t2))
+    ∧ (LIST_REL (var_rel k QG sub1 sub2) ys1 ys2)
+    ∧ (∀vs1 vs2.
+        LIST_REL (val_rel k QG) vs1 vs2
+        ⇒ exp_rel k (QL, QG) (subst1 x1 (Constructor C vs1) e1)
+                             (subst1 x2 (Constructor C vs2) e2))
+    ⇒ exp_rel k (QL, QG)
+        (Let (SOME x1) (Value $ Constructor C []) e1)
+        (Let (SOME x2) (Value $ Constructor C []) e2)
+    (*⇒ exp_rel k (QL, QG)
+        ((Let (SOME x1) (Value $ Constructor C (MAP Var ys1)) e1))
+        ((Let (SOME x2) (Value $ Constructor C (MAP Var ys2)) e2))*)
+Proof
+  cheat
+  (*rw [rel_def]
+  >> first_x_assum $ qspecl_then [`[]`, `[]`] assume_tac >> gvs []
+  >> first_x_assum $ qspecl_then [`c1 - 2`, `t1`] assume_tac >> rfs []
+  >> qexistsl [`c2 + 2`, `t2`] >> gvs []
   >> rw []
-  >- ()
-  >- rw [rel_def]
-  >- rw [rel_def]
-  >- rw [rel_def]
   >- (
-      first_x_assum $ qspecl_then [`es1`, `es2`] assume_tac >> gvs []
-     )
+      first_assum $ drule_then assume_tac
+      >> simp []
+      >> `c1 - 2 + 1 + 1 = c1` by
+          (
+          )
+     ) 
+  >- (ntac 2 (qmatch_asmsub_abbrev_tac `FST rt`
+              >> Cases_on `rt`
+              >> gvs [])
+      >> ntac 2 (qmatch_goalsub_abbrev_tac `FST rt`
+                 >> Cases_on `rt`
+                 >> gvs [])
+      >> gvs [AllCaseEqs(), eval_to'_def, check_state_def, fuel_def, trace_def,
+              rel_def]
+      >- (imp_res_tac eval_to'_zero_thm
+          >> gvs [rel_def])
+      >- (Cases_on `c1 = 1` >> gvs []   
+          >> imp_res_tac eval_to'_zero_thm
+          >> gvs [rel_def]
+          >> Cases_on `q'` >> gvs [rel_def])
+      >- (Cases_on `q` >> Cases_on `q'` >> gvs [rel_def]
+          >> qspecl_then [`k - c1`, `2`] assume_tac (cj 1 rel_add_thm)
+          >> gvs []))*)
 QED
 
 val _ = export_theory()
